ground_zero/theorems/mere_eq_lemma.lean
@@ -7,7 +7,8 @@ def to_mere_eq {α β : Sort u} (h : α = β) : ∥α = β :> Sort u∥ :=
 begin induction h, apply ground_zero.HITs.trunc.elem, reflexivity end
 
 def from_mere_eq {α β : Sort u} : ∥α = β :> Sort u∥ → α = β :=
-ground_zero.HITs.trunc.rec (begin intro x, induction x, reflexivity end)
+ground_zero.HITs.trunc.rec ground_zero.structures.prop_is_prop
+  (begin intro x, induction x, reflexivity end)
 
 lemma mere_eq {α β : Sort u} : (α = β) ≃ ∥α = β :> Sort u∥ := begin
   existsi to_mere_eq, split; existsi from_mere_eq,
